theories/Monoid/Free.v
@@ -1,0 +1,69 @@
+Require Import Blech.Defaults.
+
+Require Import Coq.Setoids.Setoid.
+Require Import Coq.Classes.SetoidClass.
+
+Require Import Blech.Bishop.
+Require Import Blech.Monoid.
+
+Import BishopNotations.
+Import MonoidNotations.
+
+Open Scope bishop_scope.
+Open Scope monoid_scope.
+
+(* The abstract AST of a monoid subject to setoid quotient. Very
+inefficient. You probably want List *)
+
+#[universes(cumulative)]
+Inductive free (S: Bishop) := η (_: S) | e | app (_ _: free S).
+
+Arguments η {S}.
+Arguments e {S}.
+Arguments app {S}.
+
+Inductive equiv {S: Bishop} : relation (free S) :=
+| reflexive: reflexive _ equiv
+| symmetric: symmetric _ equiv
+| transitive: transitive _ equiv
+
+| app_assoc f g h: equiv (app f (app g h)) (app (app f g) h)
+| app_e_left f: equiv (app e f) f
+| app_e_right f: equiv (app f e) f
+
+| app_compat: Proper (equiv ==> equiv ==> equiv) app
+.
+Existing Instance app_compat.
+
+#[global]
+#[program]
+Instance free_Setoid (S: Bishop): Setoid (free S) := {
+  equiv := equiv ;
+}.
+Next Obligation.
+Proof.
+  exists.
+  - apply reflexive.
+  - apply symmetric.
+  - apply transitive.
+Qed.
+
+#[program]
+Definition Free (S: Bishop): Monoid := {|
+  S := free S /~ free_Setoid S ;
+
+  Monoid.e := e ;
+  Monoid.app := app ;
+
+  Monoid.app_assoc := app_assoc ;
+  Monoid.app_e_left := app_e_left ;
+  Monoid.app_e_right := app_e_right ;
+  Monoid.app_compat := app_compat ;
+|}.
+
+Fixpoint ε {M: Monoid} (m: Free M): M :=
+  match m with
+  | η x => x
+  | e => Monoid.e
+  | app x y => ε x · ε y
+  end.
